src/Examples/Cells/Cells.v
@@ -5,12 +5,19 @@ Section with_semantics.
           {semantics_ok : Semantics.parameters_ok semantics}.
   Record cell := { data : Semantics.word }.
 
-  Definition cell_value (addr: address) (c: cell) : Semantics.mem -> Prop :=
+  Definition cell_value (addr: address) (c: cell)
+    : Semantics.mem -> Prop :=
     scalar addr c.(data).
 
-  Definition TwoCells a_ptr b_ptr ab : Semantics.mem -> Prop :=
-    sep (cell_value a_ptr (fst ab)) (cell_value b_ptr (snd ab)).
+  Definition OneCell c_ptr c
+    : list word -> Semantics.mem -> Prop :=
+    fun _ => cell_value c_ptr c.
+  Hint Unfold OneCell : compiler.
 
+  Definition TwoCells a_ptr b_ptr ab
+    : list word -> Semantics.mem -> Prop :=
+    fun _ =>
+      sep (cell_value a_ptr (fst ab)) (cell_value b_ptr (snd ab)).
   Hint Unfold TwoCells : compiler.
 
   Definition get c := c.(data).
@@ -19,7 +26,8 @@ Section with_semantics.
   Lemma compile_get :
     forall (locals: Semantics.locals) (mem: Semantics.mem)
            (locals_ok : Semantics.locals -> Prop)
-           tr R R' functions T (pred: T -> _ -> Prop)
+           tr retvars R R' functions
+           T (pred: T -> list word -> Semantics.mem -> Prop)
            c c_ptr c_var k k_impl,
     forall var,
       sep (cell_value c_ptr c) R' mem ->
@@ -28,6 +36,7 @@ Section with_semantics.
       (let head := v in
        find k_impl
        implementing (pred (k head))
+       and-returning retvars
        and-locals-post locals_ok
        with-locals (map.put locals var head)
        and-memory mem and-trace tr and-rest R
@@ -36,6 +45,7 @@ Section with_semantics.
        find (cmd.seq (cmd.set var (expr.load access_size.word (expr.var c_var)))
                      k_impl)
        implementing (pred (dlet head k))
+       and-returning retvars
        and-locals-post locals_ok
        with-locals locals and-memory mem and-trace tr and-rest R
        and-functions functions).
@@ -59,7 +69,8 @@ Section with_semantics.
   Lemma compile_put :
     forall (locals: Semantics.locals) (mem: Semantics.mem)
            (locals_ok : Semantics.locals -> Prop)
-           tr R R' functions T (pred: T -> _ -> Prop)
+           tr retvars R R' functions
+           T (pred: T -> list word -> _ -> Prop)
            c c_ptr c_var x x_var k k_impl,
       sep (cell_value c_ptr c) R' mem ->
       map.get locals c_var = Some c_ptr ->
@@ -70,6 +81,7 @@ Section with_semantics.
          sep (cell_value c_ptr head) R' m ->
          (find k_impl
           implementing (pred (k head))
+          and-returning retvars
           and-locals-post locals_ok
           with-locals locals
           and-memory m and-trace tr and-rest R
@@ -78,6 +90,7 @@ Section with_semantics.
        find (cmd.seq (cmd.store access_size.word (expr.var c_var) (expr.var x_var))
                      k_impl)
        implementing (pred (dlet head k))
+       and-returning retvars
        and-locals-post locals_ok
        with-locals locals and-memory mem and-trace tr and-rest R
        and-functions functions).
@@ -98,7 +111,7 @@ Section with_semantics.
       eassumption. }
   Qed.
 End with_semantics.
-Hint Unfold TwoCells : compiler.
+Hint Unfold OneCell TwoCells : compiler.
 
 Ltac cell_compile_step :=
   gen_sym_inc;
