src/Examples/ECC/Point.v
@@ -14,7 +14,7 @@ Section Compile.
   Lemma compile_point_assign :
     forall (locals: Semantics.locals) (mem: Semantics.mem)
            (locals_ok : Semantics.locals -> Prop)
-      tr R functions T (pred: T -> _ -> Prop)
+      tr retvars R functions T (pred: T -> _ -> _ -> Prop)
       (x y : Z) k k_impl,
       let v := (x mod M, y mod M)%Z in
       (let __ := 0 in (* placeholder *)
@@ -22,12 +22,14 @@ Section Compile.
        implementing (pred (dlet (x mod M)%Z
                                 (fun x => dlet (y mod M)%Z
                                                (fun y => k (x, y)))))
+       and-returning retvars
        and-locals-post locals_ok
        with-locals locals and-memory mem and-trace tr and-rest R
        and-functions functions) ->
       (let head := v in
        find k_impl
        implementing (pred (dlet head k))
+       and-returning retvars
        and-locals-post locals_ok
        with-locals locals and-memory mem and-trace tr and-rest R
        and-functions functions).
